Use strings instead of ByteString

FileNames.v
@@ -4,53 +4,49 @@ Require Import Coq.Strings.String.
 Require Import Coq.ZArith.ZArith.
 
 Require Import ByteData.
+Require Import StringOps.
 Require Import Util.
 
 Open Local Scope Z.
+Open Local Scope char.
+Open Local Scope string.
 
-Definition trimFileNamePrefix (fileName: ByteString): ByteString :=
+
+Definition trimFileNamePrefix (fileName: string): string :=
   let reversedName := rev fileName in
-  rev (takeWhile (fun (char: Z) => (negb (orb (char =? 47)    (* '/' *)
-                                              (char =? 92)))) (* '\' *)
-                 reversedName).
+  list2string
+    (rev (takeWhile (fun (char: ascii) => 
+                        (negb (orb (ascii_eqb char "/")
+                                   (ascii_eqb char "\"))))
+                   reversedName)).
 
-Fixpoint ascii2Bytes (fileName: string): ByteString :=
-  match fileName with
-  | EmptyString => nil
-  | String char tail => (Z.of_N (N_of_ascii char)) :: (ascii2Bytes tail)
-  end.
-
-Local Open Scope string_scope.
-
-Definition systemFile (fileName: ByteString) :=
+Definition systemFile (fileName: string) :=
   In (trimFileNamePrefix fileName)
-     (map ascii2Bytes ("ps" :: "netstat" :: "top" :: "ifconfig" 
-                       :: "ssh" :: "rsync" :: "ProcMon.exe"
-                       :: nil)).
+     ("ps" :: "netstat" :: "top" :: "ifconfig" :: "ssh" 
+           :: "rsync" :: "ProcMon.exe" :: nil).
 
-Definition systemFile_compute (fileName: ByteString) :=
-  existsb (listZ_eqb (trimFileNamePrefix fileName))
-          (map ascii2Bytes ("ps" :: "netstat" :: "top" :: "ifconfig" 
-                            :: "ssh" :: "rsync" :: "ProcMon.exe"
-                            :: nil)).
+Definition systemFile_compute (fileName: string) :=
+  existsb (string_eqb (trimFileNamePrefix fileName))
+          ("ps" :: "netstat" :: "top" :: "ifconfig" :: "ssh"
+                :: "rsync" :: "ProcMon.exe" :: nil).
 
-Lemma systemFile_reflection (fileName: ByteString) :
+Lemma systemFile_reflection (fileName: string) :
   systemFile_compute fileName = true -> systemFile fileName.
 Proof.
   intros. unfold systemFile_compute in H. unfold systemFile.
   apply existsb_exists in H. destruct H. destruct H.
-  apply listZ_eqb_reflection in H0. rewrite H0. auto.
+  apply string_eqb_reflection in H0. rewrite H0. auto.
 Qed.
           
 
 Lemma systemFile_ex1 : 
-  systemFile (ascii2Bytes "last/top").
+  systemFile "last/top".
 Proof.
   compute. right. right. left. reflexivity.
 Qed.
 
 Lemma systemFile_ex2 : 
-  ~(systemFile (ascii2Bytes "last/example.txt")).
+  ~(systemFile "last/example.txt").
 Proof.
   compute. intro.
   repeat (destruct H; [ inversion H | ]).
