StringOps.v
@@ -1,0 +1,105 @@
+Require Import Coq.Lists.List.
+Require Import Coq.Strings.Ascii.
+Require Import Coq.Strings.String.
+
+Open Local Scope bool.
+
+Fixpoint string2list (str: string) :=
+  match str with 
+  | EmptyString => nil
+  | String head tail => head :: (string2list tail)
+  end.
+
+Coercion string2list : string >-> list.
+
+Fixpoint list2string (lst: list ascii) :=
+  match lst with
+  | nil => EmptyString
+  | head :: tail => String head (list2string tail)
+  end.
+
+
+Definition ascii_eqb (lhs rhs: ascii) : bool :=
+  match (lhs, rhs) with
+  | (Ascii l1 l2 l3 l4 l5 l6 l7 l8, Ascii r1 r2 r3 r4 r5 r6 r7 r8) =>
+      (Bool.eqb l1 r1) && (Bool.eqb l2 r2)
+      && (Bool.eqb l3 r3) && (Bool.eqb l4 r4)
+      && (Bool.eqb l5 r5) && (Bool.eqb l6 r6)
+      && (Bool.eqb l7 r7) && (Bool.eqb l8 r8)
+  end.
+
+Lemma ascii_eqb_reflection (lhs rhs: ascii) :
+  ascii_eqb lhs rhs = true <-> lhs = rhs.
+Proof.
+  split. (* -> *)
+    intros. unfold ascii_eqb in H.
+    destruct lhs. destruct rhs.
+    apply Bool.andb_true_iff in H. destruct H. 
+    apply Bool.andb_true_iff in H. destruct H. 
+    apply Bool.andb_true_iff in H. destruct H. 
+    apply Bool.andb_true_iff in H. destruct H. 
+    apply Bool.andb_true_iff in H. destruct H. 
+    apply Bool.andb_true_iff in H. destruct H. 
+    apply Bool.andb_true_iff in H. destruct H. 
+    apply Bool.eqb_prop in H; rewrite H; clear H.
+    apply Bool.eqb_prop in H0; rewrite H0; clear H0.
+    apply Bool.eqb_prop in H1; rewrite H1; clear H1.
+    apply Bool.eqb_prop in H2; rewrite H2; clear H2.
+    apply Bool.eqb_prop in H3; rewrite H3; clear H3.
+    apply Bool.eqb_prop in H4; rewrite H4; clear H4.
+    apply Bool.eqb_prop in H5; rewrite H5; clear H5.
+    apply Bool.eqb_prop in H6; rewrite H6; clear H6.
+    reflexivity.
+  (* <- *)
+    intros. unfold ascii_eqb.
+    destruct lhs. destruct rhs. inversion H. 
+    apply Bool.andb_true_iff. split; [| apply Bool.eqb_reflx].
+    apply Bool.andb_true_iff. split; [| apply Bool.eqb_reflx].
+    apply Bool.andb_true_iff. split; [| apply Bool.eqb_reflx].
+    apply Bool.andb_true_iff. split; [| apply Bool.eqb_reflx].
+    apply Bool.andb_true_iff. split; [| apply Bool.eqb_reflx].
+    apply Bool.andb_true_iff. split; [| apply Bool.eqb_reflx].
+    apply Bool.andb_true_iff. split; [| apply Bool.eqb_reflx].
+    apply Bool.eqb_reflx.
+Qed.
+
+Fixpoint string_eqb (lhs rhs: string) :=
+  match (lhs, rhs) with
+  | (EmptyString, EmptyString) => true
+  | (String l ltail, String r rtail) =>
+      (ascii_eqb l r) && (string_eqb ltail rtail)
+  | _ => false
+  end.
+
+Lemma string_eqb_reflection (lhs rhs: string) :
+  string_eqb lhs rhs = true <-> lhs = rhs.
+Proof.
+  split. (* -> *)
+    generalize rhs.
+    induction lhs.
+      destruct rhs0.
+        reflexivity.
+        intros. compute in H. discriminate H.
+      destruct rhs0.
+        intros. compute in H. discriminate H.
+
+        intros. unfold string_eqb in H.
+          apply Bool.andb_true_iff in H. destruct H.
+          apply ascii_eqb_reflection in H. rewrite H; clear H.
+          apply IHlhs in H0. rewrite H0; clear H0.
+          reflexivity.
+  (* <- *)
+    generalize rhs.
+    induction lhs.
+      destruct rhs0.
+        reflexivity.
+        intros. discriminate H.
+      destruct rhs0.
+        intros. discriminate H.
+
+        intros. unfold string_eqb.
+          inversion H.
+          apply Bool.andb_true_iff. split.
+            apply ascii_eqb_reflection. reflexivity.
+            rewrite <- H2 at 1. apply IHlhs in H2. auto.
+Qed.
