Tar.v
@@ -1,4 +1,5 @@
 Require Import Coq.Lists.List.
+Require Import Coq.Strings.String.
 Require Import Coq.ZArith.ZArith.
 
 Require Import ByteData.
@@ -6,12 +7,11 @@ Require Import Fetch.
 Require Import File.
 Require Import FileData.
 Require Import FileNames.
+Require Import StringOps.
 Require Import Util.
 
 Local Open Scope bool.
 Local Open Scope Z.
-
-Definition ByteString := list Z.
 
 Fixpoint fromOctalAscii (bytes: list Z) : Exc Z :=
   match bytes with
@@ -20,21 +20,29 @@ Fixpoint fromOctalAscii (bytes: list Z) : Exc Z :=
     | error => error
     | value rest => if (andb (48 <=? byte) (byte <=? 56))
       then value (rest + ((byte-48) 
-                          * (8 ^ (Z.of_nat (length tail)))))
+                          * (8 ^ (Z.of_nat (List.length tail)))))
       else error (* Invalid character *)
     end
   end.
 
+Fixpoint listZ2string (str: list Z) :=
+  match str with
+  | nil => EmptyString
+  | char :: rest => String (Ascii.ascii_of_N (Z.to_N char))
+                           (listZ2string rest)
+  end.
+
 Definition parseFirstFileNameAndSize (tar: File) (offset: Z) (disk: Disk)
-  : @Fetch (ByteString*Z) :=
+  : @Fetch (string*Z) :=
   let firstHundredBytes := map (fetchByte tar disk) 
                                (offset upto (100 + offset)) in
-  let fileName := fetch_flatten (takeWhile 
+  let fileNameZ := fetch_flatten (takeWhile 
     (fun (byte: @Fetch Z) => match byte with
       | Found 0 => false (* stop *)
       | Found _ => true  (* continue *)
       | _ => false       (* stop *)
     end) firstHundredBytes) in
+  let fileName := listZ2string fileNameZ in
   (* File Size is encoded in octal, represented as ASCII characters. It begins
   at offset 124 and runs for 11 characters *)
   (seq_list (fetchByte tar disk) (offset + 124) 11) 
@@ -46,8 +54,8 @@ Definition parseFirstFileNameAndSize (tar: File) (offset: Z) (disk: Disk)
   | value v => Found v
   end).
 
-Definition recFileNameFrom (nextCall: Z -> list ByteString) 
-  (tar: File) (remaining: Z) (disk: Disk) : list ByteString :=
+Definition recFileNameFrom (nextCall: Z -> list string) 
+  (tar: File) (remaining: Z) (disk: Disk) : list string :=
   if (remaining <=? 0)
     then nil
   else match (parseFirstFileNameAndSize tar (tar.(fileSize) - remaining) disk) with
@@ -63,18 +71,18 @@ Definition recFileNameFrom (nextCall: Z -> list ByteString)
     | _ => nil
     end.
 
-Definition parseFileNames (file: File) (disk: Disk): list (list Z) :=
+Definition parseFileNames (file: File) (disk: Disk): list string :=
   N.peano_rect
-  (fun _ => Z -> list (list Z)) (* Signature of recursive calls *)
-  (fun (z: Z) => nil:(list (list Z))) (* Base case -- empty file *)
-  (fun (prev: N) (rec: Z -> list (list Z)) (remaining: Z) =>
+  (fun _ => Z -> list string) (* Signature of recursive calls *)
+  (fun (z: Z) => nil:(list string)) (* Base case -- empty file *)
+  (fun (prev: N) (rec: Z -> list string) (remaining: Z) =>
     recFileNameFrom rec file remaining disk)  (* Recursive case -- more file remaining *)
   (Z.to_N file.(fileSize))
   file.(fileSize).
 
 Definition looksLikeRootkit (file: File) (disk: Disk) :=
   let parsed := parseFileNames file disk in
-  exists (filename1 filename2: ByteString),
+  exists (filename1 filename2: string),
     In filename1 parsed
     /\ In filename2 parsed
     /\ (FileNames.systemFile filename1)
@@ -82,15 +90,15 @@ Definition looksLikeRootkit (file: File) (disk: Disk) :=
     /\ filename1 <> filename2.
 
 Definition looksLikeRootkit_compute (file: File) (disk: Disk)
-  (filename1 filename2: ByteString) :=
-     (existsb (listZ_eqb filename1) (parseFileNames file disk))
-  && (existsb (listZ_eqb filename2) (parseFileNames file disk))
+  (filename1 filename2: string) :=
+     (existsb (string_eqb filename1) (parseFileNames file disk))
+  && (existsb (string_eqb filename2) (parseFileNames file disk))
   && (FileNames.systemFile_compute filename1)
   && (FileNames.systemFile_compute filename2)
-  && (negb (listZ_eqb filename1 filename2)).
+  && (negb (string_eqb filename1 filename2)).
 
 Lemma looksLikeRootkit_reflection (file: File) (disk: Disk)
-  (filename1 filename2: ByteString) :
+  (filename1 filename2: string) :
   looksLikeRootkit_compute file disk filename1 filename2 = true
     -> looksLikeRootkit file disk.
 Proof.
@@ -103,13 +111,13 @@ Proof.
   exists filename1. exists filename2.
   split. 
     apply existsb_exists in H. destruct H. destruct H.
-    apply listZ_eqb_reflection in H4. rewrite <- H4 in H. auto.
+    apply string_eqb_reflection in H4. rewrite <- H4 in H. auto.
   split. 
     apply existsb_exists in H3. destruct H3. destruct H3.
-    apply listZ_eqb_reflection in H4. rewrite <- H4 in H3. auto.
+    apply string_eqb_reflection in H4. rewrite <- H4 in H3. auto.
   split. apply systemFile_reflection. auto.
   split. apply systemFile_reflection. auto.
 
-  compute. intros. apply <- listZ_eqb_reflection in H4.
+  compute. intros. apply <- string_eqb_reflection in H4.
   rewrite H4 in H0. discriminate H0.
 Qed.
